IL_raise.v
@@ -1,0 +1,57 @@
+Require Import List Arith.
+Require Import IL.
+
+Fixpoint raiseL (d:nat) (k:nat) (b:stmt) :=
+  match b with
+    | stmtExp x e s => stmtExp x e (raiseL d k s)
+    | stmtIf x b1 b2 => stmtIf x (raiseL d k b1) (raiseL d k b2)
+    | stmtGoto l Y => 
+      if lt_dec (counted l) d
+        then stmtGoto l Y
+        else stmtGoto (incc l k) Y
+    | stmtReturn x => stmtReturn x
+    | stmtLet s Z b => stmtLet (raiseL (S d) k s) Z (raiseL (S d) k b) 
+  end.
+
+(** raising is cummulative *)
+Lemma raiseL_cumm d k k' s
+  : raiseL d k (raiseL d k' s) = raiseL d (k+k') s.
+revert d k k'. induction s; intros; simpl; try rewrite IHs; try rewrite IHs1; try rewrite IHs2; eauto.
+destruct (lt_dec (labN l) d); simpl. destruct (lt_dec (labN l) d); try (exfalso; omega); eauto.
+destruct l; simpl. simpl in *.
+destruct (lt_dec (k' + n0) d). exfalso. omega. f_equal. f_equal. omega.
+Qed.
+
+(** another form of cummulativity *)
+Lemma raiseL_cumm' d k s
+  : raiseL (S d) k (raiseL d 1 s) = raiseL d (S k) s.
+revert d. induction s; intros; simpl; try rewrite IHs; try rewrite IHs1; try rewrite IHs2; eauto.
+destruct (lt_dec (labN l) d); simpl. destruct (lt_dec (labN l) (S d)); try (exfalso; omega); eauto.
+destruct l; simpl in * |- *.
+destruct (lt_dec (S n0) (S d)); eauto. exfalso. omega. f_equal; f_equal; omega.
+Qed.
+
+(** raising with 0 is identity *)
+Lemma raiseL_null d s
+  : raiseL d 0 s = s.
+revert d. induction s; simpl; intros; f_equal; eauto. 
+destruct l; simpl. destruct (lt_dec n d); eauto.
+Qed.
+
+(** raises can be swapped *)
+Lemma raiseL_swap a k d cont
+  : raiseL (a + 1 + d) k (raiseL d 1 cont) = raiseL d 1 (raiseL (a+d) k cont).
+revert a k d. 
+induction cont; intros; simpl; try (f_equal; now trivial). 
+destruct l; simpl. 
+destruct (lt_dec n d), (lt_dec n (a+d)); try (exfalso; omega); simpl.
+destruct (lt_dec n (a + 1 + d)), (lt_dec n d); try (exfalso; omega); trivial.
+destruct (lt_dec (S n) (a + 1 + d)), (lt_dec n d); try (exfalso; omega); trivial.
+destruct (lt_dec (S n) (a + 1 + d)), (lt_dec n d); try (exfalso; omega); trivial.
+destruct (lt_dec (k+n) d); try (exfalso; omega). 
+simpl. f_equal; f_equal; omega.
+f_equal. pose proof (IHcont1 a k (S d)). assert (S (a + 1 + d) = a + 1 + S d). omega. rewrite H0. 
+rewrite H. f_equal. f_equal. omega.
+pose proof (IHcont2 a k (S d)). assert (S (a + 1 + d) = a + 1 + S d). omega. rewrite H0. 
+rewrite H. f_equal. f_equal. omega.
+Qed.
