imp/Imp_to_ILI.v
@@ -1,0 +1,158 @@
+Require Import List Plus.
+Require Import Var Imp Imp_Types IL IL_raise IL_Types AutoIndTac EnvTy.
+
+Import ImpTS.
+
+Set Implicit Arguments.
+
+(** Control Structure Compilation *)
+
+(** In this file we compile traditional structured control flow 
+   to recursive functions *)
+
+Fixpoint compile (c:com) (cont:stmt) : stmt :=
+match c with
+  | Skip => cont
+  | Ass x e => stmtExp x e cont
+  | Seq c c' => compile c (compile c' cont)
+  | If x c c' =>
+    let cont' := raiseL 0 1 cont in (* avoid exponential blow-up by not duplicating continuations of conditionals *)
+      let s := (stmtIf x (compile c  (stmtGoto (LabI 0) nil)) 
+                         (compile c' (stmtGoto (LabI 0) nil))) in
+      stmtLet cont' nil s
+  | While x c =>
+    let cont' := raiseL 0 1 cont in
+      let body := compile c (stmtGoto (LabI 0) nil) in
+        let s := (stmtIf x body cont') in
+          stmtLet s nil (stmtGoto (LabI 0) nil)
+end.
+
+Lemma compile_typed ET c ET' (cd:comOfType ET c ET') rt
+  : forall LT cont, 
+    stmtOfType LT ET' cont rt 
+    -> stmtOfType LT ET (compile c cont) rt.
+Proof.
+  general induction cd; simpl; eauto. 
+  econstructor; eauto using stmtOfType, subEnv_update, subEnv_refl.
+
+  econstructor. instantiate (1:=ET'). firstorder.  firstorder.
+  simpl.  eapply stmtOfType_raiseL with (LT':=nil). simpl. 
+  instantiate (1:=rt). admit.
+  econstructor; eauto; try instantiate (1:=ET); firstorder. 
+  eapply IHcd1. econstructor. constructor. simpl. admit.
+  reflexivity. hnf; firstorder. 
+  eapply IHcd2. econstructor. constructor. simpl. admit.
+  reflexivity. hnf; firstorder.
+  econstructor. instantiate (1:=ET). firstorder. firstorder. 
+  econstructor. instantiate (1:=t). instantiate (1:=nil). admit.
+  instantiate (1:=rt). admit.
+  admit.
+(*  eapply IHcd. econstructor. constructor. constructor. reflexivity. hnf; firstorder.
+  eapply stmtOfType_raiseL with (LT':=nil); eauto.*)
+  econstructor. constructor. simpl. admit. reflexivity. simpl. hnf. intros. eassumption.
+Qed.
+
+Lemma raiseL_through a k c cont
+  :  raiseL a k (compile c cont) = compile c (raiseL a k cont). 
+Proof.
+  revert a k cont; induction c; intros; simpl; try rewrite IHc; try rewrite IHc1; try rewrite IHc2; eauto.
+f_equal. pose proof (raiseL_swap a k 0). 
+assert (a + 1 + 0 = S a) by omega. rewrite H0 in H. rewrite H. f_equal. f_equal. omega.
+f_equal. f_equal. pose proof (raiseL_swap a k 0). 
+assert (a + 1 + 0 = S a) by omega. rewrite H0 in H. rewrite H. f_equal. f_equal. f_equal. omega. 
+Qed.
+
+Theorem compile_correct_star E c E' : sem E c E' 
+  -> forall L cont, exists L',
+    star istep (E,  L,     compile c cont) 
+               (E',  L'++L, raiseL 0 (length L') cont).
+Proof.
+  intros A. pattern E, c, E'.
+  eapply (sem_mut_ind) with (P0:= (fun (E:env val) x c E' =>
+      forall (L : labenv) (EB:env val) cont,
+      exists L',
+        star istep (E, blockI EB
+          (stmtIf x
+            (compile c (stmtGoto (LabI 0) nil))
+            (raiseL 0 1 cont)) nil::L,
+          stmtIf x
+            (compile c (stmtGoto (LabI 0) nil))
+            (raiseL 0 1 cont))
+        (E', L'++L, raiseL 0 (length L') cont))); intros.
+
+  (* Skip *)
+  exists nil; simpl. rewrite raiseL_null; eauto using star.
+
+  (* Assignment *)
+  inv H. exists nil; simpl. rewrite raiseL_null;
+    econstructor; econstructor; eassumption; eauto using star.
+
+  (* Sequentialization *)
+  edestruct H0 with (L:=L) as [L1 HL1]; eauto.
+  edestruct H2 with (L:=L1++L) as [L2 HL2]; eauto. 
+  exists (L2++L1).
+  rewrite app_length. rewrite <- app_assoc. eapply star_trans; eauto. 
+  rewrite raiseL_through. rewrite <- raiseL_cumm. eauto.
+  
+  (* if true *)
+  edestruct H1 as [L1 HL1]; eauto.
+  instantiate (1:=(stmtGoto (LabI 0) nil)) in HL1.
+  simpl. eexists. econstructor. econstructor.
+  econstructor. econstructor. assumption. 
+  eapply star_trans. eassumption. simpl.
+  econstructor. econstructor. simpl. eapply get_shift; constructor.
+  reflexivity. simpl.
+  instantiate (1:= blockI E0 (raiseL 0 1 cont) nil::nil). simpl.
+  rewrite drop_app; simpl. (* eapply star_refl. *) admit.
+
+  (* if true *)
+  edestruct H1 as [L1 HL1]; eauto.
+  instantiate (1:=(stmtGoto (LabI 0) nil)) in HL1.
+  simpl. eexists. econstructor. constructor.
+  econstructor. eapply istepIfF. assumption. 
+  eapply star_trans. eassumption. simpl.
+  econstructor. econstructor. simpl. eapply get_shift; constructor.
+  reflexivity. simpl.
+  instantiate (1:= blockI E0 (raiseL 0 1 cont) nil::nil). simpl.
+  rewrite drop_app; simpl. (* eapply star_refl. *) admit.
+  
+  (* while case *)
+  edestruct H0. simpl. 
+  eexists. econstructor. constructor. econstructor.
+  constructor. constructor. reflexivity. simpl.
+  instantiate (1:=x0). 
+  instantiate (1:=cont) in H1. instantiate (1:=L) in H1. 
+  (* eapply H1. *) instantiate (1:=E0) in H1. admit.
+
+  (* while true *)
+  edestruct H1; eauto. 
+  edestruct H3. eexists. 
+  econstructor. constructor. assumption.
+  eapply star_trans. eapply H4. simpl.
+  econstructor. constructor. simpl. eapply get_shift. constructor.
+  simpl. reflexivity.
+  simpl. rewrite drop_app. simpl. instantiate (1:=cont) in H5. 
+  instantiate (1:=L) in H5. instantiate (1:=EB) in H5. 
+  instantiate (1:=x1).
+  admit.
+
+  (* while false *)
+  eexists (blockI EB _ nil::nil). 
+  econstructor. eapply istepIfF. assumption.
+  simpl. eapply star_refl.
+
+  assumption.
+Qed.
+
+Theorem compile_correct E c E' x : sem E c E' 
+  -> ievalsTo (E, nil, compile c (stmtReturn x)) (E'[x]). 
+Proof.
+  intros. destruct (compile_correct_star H nil (stmtReturn x)).
+  eauto using ievalsTo_star.
+Qed.
+
+(* 
+*** Local Variables: ***
+*** coq-load-path: ("../infra" "../constr" "../il" "../isa" "../") ***
+*** End: ***
+*)
